tests/lean-tests/src/lib.rs
@@ -58,7 +58,7 @@ enum WebEvent {
     PageUnload,
     // like tuple structs,
     KeyPress(char),
-    Paste(usize),
+    Paste(usize, usize),
     // or c-like structures.
     Click { x: i64, y: i64 },
 }
@@ -68,18 +68,19 @@ enum WebEvent {
 fn inspect(event: WebEvent) {
     match event {
         WebEvent::PageLoad | WebEvent::PageUnload => (),
-        // Destructure `c` from inside the `enum` variant.
         WebEvent::KeyPress(c) => (),
-        WebEvent::Paste(s) => (),
-        // Destructure `Click` into `x` and `y`.
-        WebEvent::Click { x, y } => (),
+        WebEvent::Paste(s1, s2) => (),
+        WebEvent::Click {
+            x: other_name_for_x,
+            y,
+        } => (),
     }
 }
 
 fn main_enum() {
     let pressed = WebEvent::KeyPress('x');
     // `to_owned()` creates an owned `String` from a string slice.
-    let pasted = WebEvent::Paste(56);
+    let pasted = WebEvent::Paste(56, 42);
     let click = WebEvent::Click { x: 20, y: 80 };
     let load = WebEvent::PageLoad;
     let unload = WebEvent::PageUnload;
@@ -90,4 +91,115 @@ fn main_enum() {
     inspect(load);
     inspect(unload);
     ()
+}
+
+// Tuples
+
+// Manual
+struct T0();
+struct T1<A>(A);
+struct T2<A, B>(A, B);
+
+fn f_manual_tuples() {
+    let t0 = T0();
+    let t1 = T1(32);
+    let t2 = T2(1, 2);
+    ()
+}
+
+// Builtin
+fn main_tuples() {
+    let t0: () = ();
+    let t1: (usize,) = (42,);
+    let t2: (usize, isize) = (42, 41);
+    let t3: (u32, u64, u8) = (1, 2, 3);
+}
+
+// Structs
+// taken (and adapted) from https://doc.rust-lang.org/rust-by-example/custom_types/structs.html
+
+#[derive(Debug)]
+struct Person {
+    name: String,
+    age: u8,
+}
+
+// A unit struct
+struct Unit;
+
+// A tuple struct
+struct Pair(i32, i64);
+
+// A struct with two fields
+struct Point {
+    x: i64,
+    y: i64,
+}
+
+// Structs can be reused as fields of another struct
+struct Rectangle {
+    // A rectangle can be specified by where the top left and bottom right
+    // corners are in space.
+    top_left: Point,
+    bottom_right: Point,
+}
+
+fn main_structs() {
+    // Create struct with field init shorthand
+    let name = String::from("Peter");
+    let age = 27;
+    let peter = Person { name, age };
+
+    // Instantiate a `Point`
+    let point: Point = Point { x: 5, y: 0 };
+    let another_point: Point = Point { x: 10, y: 0 };
+
+    // Access the fields of the point
+    let _ = point.x;
+    let _ = point.y;
+
+    // Make a new point by using struct update syntax to use the fields of our
+    // other one
+    let bottom_right = Point {
+        x: 10,
+        ..another_point
+    };
+
+    // `bottom_right.y` will be the same as `another_point.y` because we used that field
+    // from `another_point`
+
+    // Access the fields of the point
+    let _ = bottom_right.x;
+    let _ = bottom_right.y;
+
+    // Destructure the point using a `let` binding
+    let Point {
+        x: left_edge,
+        y: top_edge,
+    } = point;
+
+    let _rectangle = Rectangle {
+        // struct instantiation is an expression too
+        top_left: Point {
+            x: left_edge,
+            y: top_edge,
+        },
+        bottom_right: bottom_right,
+    };
+
+    // Instantiate a unit struct
+    let _unit = Unit;
+
+    // Instantiate a tuple struct
+    let pair = Pair(1, 0);
+
+    // Access the fields of a tuple struct
+    let _ = pair.0;
+    let _ = pair.1;
+
+    // Destructure a tuple struct
+    let Pair(integer, decimal) = pair;
+
+    let _ = integer;
+    let _ = decimal;
 }
